theories/Prover.v
@@ -4,7 +4,7 @@ Require Extraction.
 Require Import Int63.
 
 Extract Constant int => "Uint63.t".
-Extract Constant Int63.ltb => "Uint63.lt".
+Extract Constant Uint63.ltb => "Uint63.lt".
 Extract Constant Int63.eqb => "Uint63.equal".
 Extract Constant Int63.add => "Uint63.add".
 Extract Constant Int63.lsl => "Uint63.l_sl".
